

L24 - 10-23 SLLN proof

Wednesday, October 23, 2024 11:30 AM

SLLN: $\{x_i, x_k\}_{k \geq 1}$ ~~i.i.d.~~ ^{pairwise} $E|X| < \infty$, $E(X) = \mu$

then $\frac{S_n}{n} \xrightarrow[n \rightarrow \infty]{a.s.} \mu$ $S_n = \sum_{k=1}^n x_k$, $n=1,2,\dots$

First observed WLOG $X \geq 0$ a.s.

$$X_k = X_k^+ - X_k^- \quad , \quad X_k^+ = \max(X, 0), \quad E(X^+) < \infty$$

$\{X_k^+, X_k^-\}$ i.i.d.

$$S_n^+ \equiv \sum_{k=1}^n X_k^+$$

$$\frac{S_n^+}{n} - \frac{S_n^-}{n} = \frac{S_n}{n}$$

Step 1 $Y_k = X_k \mathbb{1}_{\{|X_k| \leq k\}}$, $k=1,2,\dots$

$$\sum_{k=1}^{\infty} P(X_k \neq Y_k) = \sum_{k=1}^{\infty} P(|X_k| > k) = \sum_{k=1}^{\infty} P(|X| > k) \approx \int_0^{\infty} P(|X| \geq x) dx = E|X| < \infty$$

By BCT: $P(X_k \neq Y_k \text{ i.o.}) = 0$

$$\Rightarrow \sum_{k=1}^n Y_k \xrightarrow[n \rightarrow \infty]{a.s.} E(X) \quad \text{then} \quad \frac{S_n}{n} \xrightarrow[n \rightarrow \infty]{a.s.} \mu$$

$P(X_k \neq Y_k \text{ i.o.}) \rightarrow X_k = Y_k \text{ a.s.}$

As i.d.e.

Levental named

Def. let $a_n \uparrow \infty$ we say $\{a_n\}_{n \geq 1}$ is "Good"

$$\text{if } \sum_{n=m}^{\infty} a_n^{-2} \leq C_m \cdot a_m^{-2}, \quad m=1,2,\dots$$

Ex: $a_n = \frac{1}{n^{1/p}}$, $0 < p < 2$ more generally:

if $\frac{a_n}{n^{1/p}}$ is non-decreasing, then $\{a_n\}$ "is Good"

"note $\frac{1}{n^{1/p}}$ is decreasing."

Lemma

let $Y_n = X_n \cdot \mathbb{1}_{\{|X_n| \leq a_n\}}$, $n \geq 1$ in this case $a_n = n$.

Assume $\sum_{n=1}^{\infty} P(|X| > a_n) < \infty$

Then $\sum_{n=1}^{\infty} \frac{E(Y_n^2)}{a_n^2} < \infty$

Step 2. $\sum_{k=1}^{\infty} \frac{E(Y_k^2)}{k^2} < \infty$

"in the book he uses diff proof, not the following"

$$\sum_{n=1}^{\infty} \frac{E(Y_n^2)}{a_n^2} = \sum_{n=1}^{\infty} a_n^{-2} \sum_{m=1}^n E(X^2; a_{m-1} < |X| \leq a_m)$$

note $1 \leq m \leq n < \infty$ $1 \leq n < \infty$



$$\sum_{n=1}^{\infty} \left[\sum_{m=n}^{\infty} a_n^{-2} \right] E(X^2; a_{m-1} < |X| \leq a_m)$$

$$\leq \sum_{m=1}^{\infty} C \cdot m \cdot \underbrace{a_m^{-2}}_{\text{constant}} E(X^2; a_{m-1} < |X| \leq a_m)$$

$$\leq C \sum_{m=1}^{\infty} m P(a_{m-1} < |X| \leq a_m) = C \sum_{m=0}^{\infty} P(|X| > a_m) < \infty$$

note $\sum_{m=1}^{\infty} \left(\sum_{k=1}^m \right) (P(\dots)) \stackrel{\text{Fubini?}}{=} C \sum_{k=1}^{\infty} \sum_{m=k}^{\infty} P(\dots)$

$$= C \sum_{k=1}^{\infty} P(|X| > a_{m-1}) < \infty$$

"similar to find $P(X > x) = \sum_x x P(X=x)$ "

Step 3 let $T_n \equiv \sum_{k=1}^n Y_k$, $n \geq 1$

$$\forall \alpha > 1 \quad \text{we get} \quad \frac{T_{\alpha^n} - E(T_{\alpha^n})}{\alpha^n} \xrightarrow[n \rightarrow \infty]{\text{a.s.}} 0.$$

if α is $\mathbb{Q} \setminus \mathbb{Z}$ get messy

Proof ($\alpha \geq 2$)

"chev-bon-yan" proof.

Claim $U_n \equiv \sum_{k=2^{n-1}+1}^{2^n} \frac{Y_k - E(Y_k)}{2^n} \xrightarrow[n \rightarrow \infty]{\text{a.s.}} 0$

we will show: $\sum_{n=1}^{\infty} E(U_n^2) < \infty$ ($\Rightarrow \sum_{n=1}^{\infty} U_n^2 < \infty$ a.s.)

implies $U_n^2 \xrightarrow[n \rightarrow \infty]{\text{a.s.}} 0$

$$= U_n \xrightarrow[n \rightarrow \infty]{\text{a.s.}} 0$$

$$\dots \quad |T_n - E(T_n)| \leq \sum_{k=1}^{2^{n-1}} |Y_k - E(Y_k)| \leq 4 \sum_{k=1}^{2^{n-1}} \frac{\text{Var}(Y_k)}{1/2}$$

$$= U_n \xrightarrow[n \rightarrow \infty]{} 0$$

$$\text{then } E(U_n^2) = \text{Var} \left(\sum_{k=2^{n+1}}^{2^{n+1}} \frac{Y_k - E(Y_k)}{2^n} \right) \leq 4 \sum_{k=2^{n+1}}^{2^{n+1}} \frac{\text{Var}(Y_k)}{k^2}$$

$$\left| \begin{array}{l} 2^n < 2^{n+1} \leq k \leq 2^{n+1} \\ (2^n)^2 \leq k^2 \leq (2^{n+1})^2 = (2^n)^2 \cdot 4 \end{array} \right.$$

$$\leq 4 \cdot \sum_{k=2^{n+1}}^{2^{n+1}} \frac{\text{Var}(Y_k)}{k^2}$$

$$\sum_{n=1}^{\infty} E(U_n^2) \leq 4 \sum_{n=1}^{\infty} \sum_{k=2^{n+1}}^{\infty} \frac{E(Y_k^2)}{k^2} = 4 \sum_{k=1}^{\infty} \frac{E(Y_k^2)}{k^2}$$

$$\left(\begin{array}{l} T_{2^n} = \sum_{k=1}^{2^{n+1}} \frac{Y_k - E(Y_k)}{2^n} \\ \sum_{k=0}^n 2^k = 2^{n+1} - 1 \end{array} \right.$$

$$\frac{T_{2^n} - E(T_{2^n})}{2^n} = \sum_{m=1}^{2^n} \frac{2^m}{2^n} U_m \xrightarrow[n \rightarrow \infty]{\text{a.s.}} 0$$

we know $U_n \rightarrow 0$ A.S.

so for small n this is 0.

Then for large n $U_m \rightarrow 0$.

$\therefore 0$

$$\frac{E(T_{2^n})}{2^n} = \sum_{k=1}^{2^n} \frac{E(Y_k)}{2^n} \xrightarrow[n \rightarrow \infty]{} E(X)$$

$$E(Y_k) = E(X; |X| \leq k) \xrightarrow[k \rightarrow \infty]{\text{B\ddot{o}rj\ddot{e}r's PCT}} E(X)$$

$$\frac{T_{2^n} - E(T_{2^n})}{2^n} \xrightarrow[n \rightarrow \infty]{\text{a.s.}} 0$$

$$\Rightarrow \frac{T_{2^n}}{2^n} \xrightarrow[n \rightarrow \infty]{\text{a.s.}} M$$